

Please find below the set of algebraic equations for the flattened fibonacci\_gen  
CBD:

$$\left\{ \begin{array}{lcl} \text{var}(b.O_1)^{[s+1]} & = & \text{var}(a.I_C)^{[0]} \\ \text{var}(c.O_1)^{[s+1]} & = & \text{var}(a.I_1)^{[s]} \\ \text{var}(e.O_1)^{[s+1]} & = & \text{var}(d.I_C)^{[0]} \\ \text{var}(a.O_1)^{[s+1]} & = & \text{var}(d.I_1)^{[s]} \\ \text{var}(g.O_1)^{[s+1]} & = & \text{var}(f.I_C)^{[0]} \\ \text{var}(c.O_1)^{[s+1]} & = & \text{var}(f.I_1)^{[s]} \\ \text{var}(a.O_1)^{[s+1]} & = & \text{var}(c.I_1)^{[s+1]} \\ \text{var}(d.O_1)^{[s+1]} & = & \text{var}(c.I_2)^{[s+1]} \\ \text{var}(i.O_1)^{[s+1]} & = & \text{var}(j.I_1)^{[s+1]} \\ \text{var}(k.O_1)^{[s+1]} & = & \text{var}(j.I_2)^{[s+1]} \\ \text{var}(j.O_1)^{[s+1]} & = & \text{var}(l.I_1)^{[s+1]} \\ \text{var}(m.O_1)^{[s+1]} & = & \text{var}(l.I_2)^{[s+1]} \\ \text{var}(j.O_1)^{[s+1]} & = & \text{var}(k.I_1)^{[s+1]} \\ \text{var}(h.O_1)^{[s+1]} & = & \text{var}(m.I_1)^{[s+1]} \\ \text{var}(h.O_1)^{[s+1]} & = & \text{var}(n.I_1)^{[s+1]} \\ \text{var}(i.O_1)^{[s+1]} & = & \text{var}(n.I_2)^{[s+1]} \\ \text{var}(j.O_1)^{[s+1]} & = & \text{var}(b.I_1)^{[s+1]} \\ \text{var}(l.O_1)^{[s+1]} & = & \text{var}(e.I_1)^{[s+1]} \\ \text{var}(n.O_1)^{[s+1]} & = & \text{var}(g.I_1)^{[s+1]} \\ \text{var}(f.O_1)^{[s+1]} & = & \text{var}(o.I_1)^{[s+1]} \\ \text{var}(a.O_1)^{[s+1]} & = & \text{var}(a.I_1)^{[s]} \\ \text{var}(a.O_1)^{[0]} & = & \text{var}(a.I_C)^{[0]} \\ \text{var}(d.O_1)^{[s+1]} & = & \text{var}(d.I_1)^{[s]} \\ \text{var}(d.O_1)^{[0]} & = & \text{var}(d.I_C)^{[0]} \\ \text{var}(f.O_1)^{[s+1]} & = & \text{var}(f.I_1)^{[s]} \\ \text{var}(f.O_1)^{[0]} & = & \text{var}(f.I_C)^{[0]} \\ \text{var}(c.O_1)^{[s+1]} & = & \text{var}(c.I_1)^{[s+1]} + \text{var}(c.I_2)^{[s+1]} \\ \text{var}(h.O_1)^{[s+1]} & = & 1.0 \\ \text{var}(i.O_1)^{[s+1]} & = & 2.0 \\ \text{var}(j.O_1)^{[s+1]} & = & \text{var}(j.I_1)^{[s+1]} + \text{var}(j.I_2)^{[s+1]} \\ \text{var}(l.O_1)^{[s+1]} & = & \text{var}(l.I_1)^{[s+1]} + \text{var}(l.I_2)^{[s+1]} \\ \text{var}(k.O_1)^{[s+1]} & = & -\text{var}(k.I_1)^{[s+1]} \\ \text{var}(m.O_1)^{[s+1]} & = & -\text{var}(m.I_1)^{[s+1]} \\ \text{var}(n.O_1)^{[s+1]} & = & \frac{1}{(\text{var}(n.I_1)^{[s+1]}) \text{var}(n.I_2)^{[s+1]}} \end{array} \right.$$

Given:

- Block **D1** is represented by variable **a**
- Block **conditions.OUT1** is represented by variable **b**
- Block **sum** is represented by variable **c**
- Block **D2** is represented by variable **d**
- Block **conditions.OUT2** is represented by variable **e**
- Block **D3** is represented by variable **f**
- Block **conditions.OUT3** is represented by variable **g**
- Block **conditions.one** is represented by variable **h**
- Block **conditions.two** is represented by variable **i**
- Block **conditions.sum1** is represented by variable **j**
- Block **conditions.neg1** is represented by variable **k**
- Block **conditions.sum2** is represented by variable **l**
- Block **conditions.neg2** is represented by variable **m**
- Block **conditions.root** is represented by variable **n**
- Block **OutFib** is represented by variable **o**